hw6 seems to be done

Assignment 6/Homework6.dfy
@@ -3,54 +3,49 @@ datatype List<T> = Nil | Cons(T, List<T>)
 
 function flatten<T>(tree:Tree<T>):List<T>
 {
-    match tree
-    case Leaf => Nil
-    case Node(leftTree, rightTree, x) => append(flatten(leftTree), Cons(x, flatten(rightTree)))
+        match tree
+        case Leaf => Nil
+        case Node(leftTree, rightTree, x) => Cons(x, append(flatten(leftTree), flatten(rightTree)))
 }
 
 function append<T>(xs:List<T>, ys:List<T>):List<T>
 {
-    match xs
-    case Nil => ys
-    case Cons(x, xs') => Cons(x, append(xs', ys))
+        match xs
+        case Nil => ys
+        case Cons(x, xs') => Cons(x, append(xs', ys))
 }
 
 function treeContains<T>(tree:Tree<T>, element:T):bool
 {
-	match tree
-    case Leaf => false
-    case Node(leftTree, rightTree, x) => treeContains(leftTree, element) || treeContains(rightTree, element) || x == element
+        match tree
+        case Leaf => false
+        case Node(leftTree, rightTree, x) => treeContains(leftTree, element) || treeContains(rightTree, element) || x == element
 }
 
 function listContains<T>(xs:List<T>, element:T):bool
 {
-	match xs
-    case Nil => false
-    case Cons(x, xs') => listContains(xs', element) || x == element
+        match xs
+        case Nil => false
+        case Cons(x, xs') => listContains(xs', element) || x == element
 }
 
+
+lemma appendListContains<T>(xs:List<T>, ys:List<T>, element:T)
+ensures listContains(append(xs, ys), element) <==> listContains(xs, element) || listContains(ys, element) 
+{
+        match xs
+        case Nil => {}
+        case Cons(x, xs') => {}
+}
 
 lemma sameElements<T>(tree:Tree<T>, element:T)
 ensures treeContains(tree, element) <==> listContains(flatten(tree), element)
 {
 	match tree
-    case Leaf => {}
-    case Node(leftTree, rightTree, x) => {
-        sameElements(leftTree, x);
-        sameElements(rightTree, x);
-
-        assert treeContains(tree, element)
-            == (treeContains(leftTree, element) || treeContains(rightTree, element) || x == element)
-            == (listContains(flatten(leftTree), element) || listContains(flatten(rightTree), element) || x == element)
-            == (listContains(flatten(leftTree), element) || (listContains(Cons(x, flatten(rightTree)), element)))
-            == listContains(append(flatten(leftTree), Cons(x, flatten(rightTree))), element)
-            == listContains(flatten(tree), element);
-    
-        assert listContains(flatten(tree), element)
-            == listContains(append(flatten(leftTree), Cons(x, flatten(rightTree))), element)
-            == (listContains(flatten(leftTree), element) || listContains(Cons(x, flatten(rightTree)), element))
-            == (listContains(flatten(leftTree), element) || listContains(flatten(rightTree), element) || x == element)
-            == (treeContains(leftTree, element) || treeContains(rightTree, element) || x == element)
-            == treeContains(tree, element);
-    }
+        case Leaf => {}
+        case Node(leftTree, rightTree, x) => {
+            sameElements(leftTree, x);
+            sameElements(rightTree, x);
+            appendListContains(flatten(leftTree), flatten(rightTree), element);
+        }
 }
