Assignment 6/ExtraCredit.dfy
@@ -12,12 +12,14 @@ function eval(e:Exp, store:map<string, int>):int
 //fill this function in to make optimizeFeatures work
 function optimize(e:Exp):Exp
 {
-	e
+	match e
+	case Const(int) => 
+	case Var(string)
 }
 
 //as you write optimize this will become unproved
 //you must write proof code so that Dafny can prove this
- method optimizeCorrect(e:Exp, s:map<string, int>)
+method optimizeCorrect(e:Exp, s:map<string, int>)
 ensures eval(e,s) == eval(optimize(e), s)
 {
 
